examples/incr_faa/ClientIA.v
@@ -5,20 +5,8 @@ From iris Require Import frac_auth numbers.
 
 Require Import Common Mod ltac2_lib.
 
-Program Global Instance fspec_winv_precond
-    `{!crisG Γ Σ α β τ _S _I, !concG, !newschG} (fsp : fspec) N stid m arg varg :
-  WP (precond (fspec_sch fsp) (N, stid) m arg varg) :=
-  {| WP_space := ↑N; WP_remainder := Tid m.1 stid ∗ (precond fsp (N, m.1) m.2 arg varg) |}.
-Next Obligation. intros; destruct m; iSplit; iIntros "[$ $]". Qed.
-
-Program Global Instance fspec_winv_postcond
-    `{!crisG Γ Σ α β τ _S _I, !concG, !newschG} (fsp : fspec) N stid m arg varg :
-  WP (postcond (fspec_sch fsp) (N, stid) m arg varg) :=
-  {| WP_space := ↑N; WP_remainder := Tid m.1 stid ∗ (postcond fsp (N, m.1) m.2 arg varg) |}.
-Next Obligation. intros; destruct m; iSplit; iIntros "[$ $]". Qed.
-
 Ltac simpl_sp :=
-  match goal with
+  try match goal with
   | H : ?sp1 ⊆ ?sp2 |- context [?sp2 !! ?key] =>
     unshelve erewrite (lookup_weaken sp1 sp2 key _ _ H);
     [|rewrite /sp1; simpl_map; reflexivity|]
@@ -29,42 +17,43 @@ Module ClientIA. Section ClientIA.
   Import ClientA.
   Context `{!crisG Γ Σ α β τ _S _I, !concG, !memG, !newschG, !incrG}.
 
+  Context (N : namespace).
   Context (sp_user sp : specmap).
-  Context (Hclient : ClientA.sp ⊆ sp_user).
-  Context (Hsch : SchA.sp sp_user ⊆ sp).
+  Context (Hclient : ClientA.sp N ⊆ sp_user).
+  Context (Hsch : SchA.sp sp_user (↑N) ⊆ sp).
 
-  Local Definition IstFull := (IstProd (IstSB (ClientA.t sp).(Mod.scopes) IstTrue) IstEq).
-  Local Definition MA := (ClientA.t sp ★ MemA.t sp).
+  Local Definition IstFull := (IstProd (IstSB (ClientA.t N sp).(Mod.scopes) IstTrue) IstEq).
+  Local Definition MA := (ClientA.t N sp ★ MemA.t sp).
   Local Definition MI := ((ClientI.t ★ FaaA.t) ★ MemA.t sp).
 
   Lemma f_spawnable γ v bofs :
-    SchA.fn_spawnable sp_user (IncrHdr.incr)
-      (λ N varg arg,
+    ⊢ SchA.fn_spawnable sp_user (IncrHdr.incr)
+      (λ varg arg,
         ⌜varg = arg ∧ varg = ([Vptr bofs]↑↑)⌝
         ∗ counter γ (1/2) v
         ∗ incr_inv 0 N γ bofs)%I
       (λ vret ret,
         existT 0 ((⌜vret = ret ∧ vret = tt↑↑⌝ ∗ counter_syn γ (1/2) (v + 2))%SAT)).
   Proof using Hclient.
-    eexists; split.
-    { simpl_sp. refl. }
-    intros [N ?] mtid; exists (mtid, (bofs, v, γ)); unfold_pre_post; split; i.
-    - iIntros "[$ [$ [% [% [[-> ->] [[-> ->] [$ $]]]]]]]". done.
-    - iIntros "[$ [$ [[-> ->] ?]]] !>". iExists _, _; iSplitR; eauto.
-      SL_red. iSplitR; eauto.
+    iExists _; iSplitL.
+    { simpl_sp. eauto. }
+    iApply SchA.fspec_sch_spawnable; first done.
+    iIntros ([]); iExists (bofs, v, γ); unfold_pre_post.
+    iIntros (varg arg) "[%va [%sarg [[% %] [% $]]]]"; des; clarify.
+    iIntros "!>"; iSplit; first done; iIntros "%% [[-> ->] ?] !>"; iExists _, _; iSplit; eauto.
+    solve_base_sl_red; iSplit; done.
   Qed.
 
   Ltac sch_yield_ir H1 H2 :=
-    iApply (wsim_yield_tgt); [ss|ss|simpl_map; simpl_sp]; iFrame H1; iFrame H2;
-      iSplit; [try done|clear_st; iIntros (??) H1;
-      let H2' := eval compute in ("[_ " ++ H2 ++ "]")%string in iIntros H2'].
+    let H2' := eval compute in (H1 ++ " " ++ H2)%string in
+    (norm_l with do 1 (iApply (wsim_yield_tgt_ir); [simpl_sp; ss|simpl_sp; ss|ss|ss|iFrame H2']));
+    clear_st; iIntros (??) H2'.
 
   Lemma incr_simF : ISim.sim_fun open MA MI IstFull (Some IncrHdr.incr).
   Proof using Hsch Hclient.
     iStartSim.
 
-    steps_l. destruct _q as [N stid].
-    steps_l. destruct _q as [mtid [[[blk ofs] v]]]; s.
+    steps_l. destruct _q as [[stid mtid] [[[blk ofs] v]]]; rename _q0 into varg.
     iDestruct "ASM" as "[TID [[-> ->] [C #INV]]]". hss_l; hss_r.
 
     steps_l. steps_r. hss_l. hss_r. steps_l. steps_r.
@@ -76,28 +65,24 @@ Module ClientIA. Section ClientIA.
     steps_r. inline_r. steps_r. hss_r. steps_r.
     sch_yield_ir "IST" "TID".
 
-    rewrite /incr_inv.
-    iInv "INV" as "I" "IA". SL_red.
-    iDestruct "I" as (x) "PT". SL_red. iDestruct "PT" as "[PT CA]".
+    iInv "INV" as "[%x [PT CA]]" "IA".
 
     (* operational atomicity here *)
     forces_r; iFrame "PT"; steps_r.
 
     iMod (counter_incr 1 with "[C CA]") as "[C CA]"; first iFrame.
     iMod ("IA" with "[GRT CA]") as "_".
-    { iExists (x + 1)%Z; SL_red; ss; iFrame. }
+    { iExists (x + 1)%Z; solve_base_sl_red; iFrame. }
     sch_yield_ir "IST" "TID".
 
-    rewrite /incr_inv.
-    iInv "INV" as "I" "IA". SL_red.
-    iDestruct "I" as (y) "PT". SL_red. iDestruct "PT" as "[PT CA]".
+    iInv "INV" as "[%y [PT CA]]" "IA".
 
     (* operational atomicity here *)
     forces_r; iFrame "PT"; steps_r.
 
     iMod (counter_incr 1 with "[C CA]") as "[C CA]"; first iFrame.
     iMod ("IA" with "[GRT CA]") as "_".
-    { iExists (y + 1)%Z; SL_red; ss; iFrame. }
+    { iExists (y + 1)%Z; solve_base_sl_red; iFrame. }
     sch_yield_ir "IST" "TID".
 
     steps_r; hss_r; steps_r.
@@ -114,7 +99,7 @@ Module ClientIA. Section ClientIA.
   Proof using Hsch Hclient.
     iStartSim.
 
-    steps_l. destruct _q as [N stid]. steps_l. destruct _q as [mtid []]; s.
+    steps_l. destruct _q as [[stid mtid] []]; s.
     iDestruct "ASM" as "[TID ->]".
     rewrite /main /ClientI.main.
 
@@ -140,7 +125,7 @@ Module ClientIA. Section ClientIA.
     { apply frac_auth_valid; ss. }
     iMod (inv_alloc (ccounter_syn 0 γc (blk, 0%Z)) _ _ _ (N_main N) with "[map A]") as "#I"; eauto.
     { apply nclose_subseteq. }
-    { rewrite /ccounter_syn; SL_red; iExists 0; SL_red; iFrame. }
+    { solve_base_sl_red; iFrame. }
     iPoseProof (counter_op with "[F]") as "[F1 F2]".
     { rewrite -Qp.half_half -{2}(Z.add_0_r 0%Z). iApply "F". }
 
@@ -149,11 +134,11 @@ Module ClientIA. Section ClientIA.
     (* src/tgt spawns *)
     rewrite /Sch.spawn; steps_r; steps_l. simpl_sp.
     force_l (_, _); forces_l; iSplitL "F1".
-    { iExists _, _, _; iSplit.
-      { iPureIntro; split; [done|split; [done|]]. eapply f_spawnable. }
-      ss. iFrame; iSplit; eauto.
+    { iExists _, _, _; iSplit; eauto.
+      iSplitR; first iApply f_spawnable.
+      iFrame; eauto.
     }
-    steps_l. call "IST". clear_st. iIntros (ret st_src st_tgt) "IST".
+    steps_l. call "IST". clear_st. iIntros (ret ??) "IST".
     steps_l. iDestruct "ASM" as "[% [[-> ->] Handle]]". hss_l. steps_l.
     steps_r. hss_r. steps_r.
     sch_yield_ir "IST" "TID".
@@ -161,35 +146,34 @@ Module ClientIA. Section ClientIA.
 
     rewrite /Sch.spawn; steps_r; steps_l. simpl_sp.
     force_l (_, _); forces_l; iSplitL "F2".
-    { iExists _, _, _; iSplit.
-      { iPureIntro; split; [done|split; [done|]]. eapply f_spawnable. }
-      ss. iFrame; iSplit; eauto.
+    { iExists _, _, _; iSplit; eauto.
+      iSplitR; first iApply f_spawnable.
+      iFrame; eauto.
     }
-    steps_l. call "IST". clear_st. iIntros (ret st_src st_tgt) "IST".
+    steps_l. call "IST". clear_st. iIntros (ret ??) "IST".
     steps_l. iDestruct "ASM" as "[% [[-> ->] Handle2]]". hss_l. steps_l.
     steps_r. hss_r. steps_r.
     sch_yield_ir "IST" "TID".
     sch_yield_l.
 
     rewrite /Sch.join; steps_r; steps_l. simpl_sp.
-    force_l (_, _); forces_l. iFrame "TID Handle"; iSplit; [eauto|]. steps_l.
-    call "IST". clear_st. iIntros (ret st_src st_tgt) "IST".
+    force_l (_, _, _); forces_l. iFrame "TID Handle"; iSplit; [eauto|]. steps_l.
+    call "IST". clear_st. iIntros (ret ??) "IST".
     steps_l. iDestruct "ASM" as "[TID [% [% [[-> ->] ASM]]]]".
-    SL_red. iDestruct "ASM" as "[[-> ->] Q]".
+    solve_base_sl_red. iDestruct "ASM" as "[[-> ->] Q]".
     hss_l. steps_l. steps_r. hss_r. steps_r.
     sch_yield_ir "IST" "TID".
     sch_yield_l.
 
     rewrite /Sch.join; steps_r; steps_l. simpl_sp.
-    force_l (_, _); forces_l. iFrame "TID Handle2"; iSplit; [eauto|]. steps_l.
-    call "IST". clear_st. iIntros (ret st_src st_tgt) "IST".
+    force_l (_, _, _); forces_l. iFrame "TID Handle2"; iSplit; [eauto|]. steps_l.
+    call "IST". clear_st. iIntros (ret ??) "IST".
     steps_l. iDestruct "ASM" as "[TID [% [% [[-> ->] ASM]]]]".
-    SL_red. iDestruct "ASM" as "[[-> ->] Q2]".
+    solve_base_sl_red. iDestruct "ASM" as "[[-> ->] Q2]".
     hss_l. steps_l. steps_r. hss_r. steps_r.
     sch_yield_ir "IST" "TID".
 
-    iInv "I" as "INV" "INVA"; iEval (SL_red) in "INV"; iDestruct "INV" as "[%x INV]".
-    iEval (SL_red) in "INV". iDestruct "INV" as "[PT C]".
+    iInv "I" as "[%x [PT C]]" "INVA".
     iCombine "C Q Q2" as "C" gives %[_ WF%frac_auth_agree]. inv WF; ss.
     iDestruct "C" as "[CA CF]".
 
@@ -197,8 +181,7 @@ Module ClientIA. Section ClientIA.
     iApply (wsim_mem_load with "[PT]"); [ss|ss|].
     iIntros "PT". steps_r. hss_r. steps_r.
 
-    iMod ("INVA" with "[CA PT]") as "_".
-    { SL_red. iExists _; SL_red; iFrame. }
+    iMod ("INVA" with "[CA PT]") as "_"; first solve_base_sl_red; iFrame.
 
     sch_yield_ir "IST" "TID". steps_r.
     sch_yield_ir "IST" "TID". 
@@ -223,12 +206,12 @@ End ClientIA.
 Section ctxr.
   Context `{!crisG Γ Σ α β τ _S _I, !concG, !memG, !newschG, !incrG}.
 
-  Definition ctxr (sp_user sp : specmap) :
-    ClientA.sp ⊆ sp_user →
-    (SchA.sp sp_user) ⊆ sp →
+  Definition ctxr (N : namespace) (sp_user sp : specmap) :
+    ClientA.sp N ⊆ sp_user →
+    (SchA.sp sp_user (↑N)) ⊆ sp →
     ctx_refines
-      (ClientA.t sp ★ MemA.t sp, emp%I)
-      (ClientI.t    ★ FaaA.t ★ (MemA.t sp), emp%I).
+      (ClientA.t N sp ★ MemA.t sp, emp%I)
+      (ClientI.t      ★ FaaA.t ★ (MemA.t sp), emp%I).
   Proof using.
     etrans; cycle 1. { do 2 ctxr_rotate. ctxr_refl. }
     eset (GRP := ClientI.t ★ _).
