examples/incr_faa/FaaA.v
@@ -28,8 +28,7 @@ Module FaaA. Section FaaA.
     SMod.fnsems := fnsems;
     SMod.initial_st := ∅;
   |}.
-  Solve All Obligations with try done.
-  Next Obligation. rewrite ?omap_insert /= omap_empty. mod_tac scope_solver. Qed.
+  Solve All Obligations with mod_tac.
 
   Definition t : Mod.t := SMod.to_mod ∅ smod.
 End FaaA. End FaaA.
