scheduler/SchIAproof.v
@@ -44,14 +44,15 @@ Module SchIA. Section sim.
     iStartSim.
     step_l. destruct _q.
     steps_l.
-    iDestruct "ASM" as "[%stid [%pre [%postS [%fvarg [%varg [%fn [%mtid [[-> [-> %Hspawn]] ASM]]]]]]]]".
-    iDestruct "ASM" as "[? [TidFrag [Pre JoinFrag]]]".
+    iDestruct "ASM" as "[%stid [%pre [%postS [%fvarg [%varg [%fn [%mtid [[-> ->] ASM]]]]]]]]".
+    iDestruct "ASM" as "[Spawn [W [TidFrag [Pre JoinFrag]]]]".
     hss_l; hss_r.
 
     steps_l. steps_r.
-    destruct Hspawn as [fsp [Hfind Hspawn]]; erewrite lookup_weaken; eauto using Hfind.
-    destruct (Hspawn (stid, mtid)) as [x [Hpre Hpost]].
-    iPoseProof (Hpre with "[-IST JoinFrag]") as "> Post".
+    iDestruct "Spawn" as "[%fsp [%Hfind Spawn]]".
+    erewrite lookup_weaken; eauto using Hfind.
+    iDestruct ("Spawn" $! (stid, mtid, tt)) as "[%x Hspawn]".
+    iPoseProof ("Hspawn" with "[-IST JoinFrag]") as "> [Pre Post]".
     { unfold_pre_post; iFrame; eauto. }
     force_l x. forces_l. iFrame.
 
@@ -60,7 +61,7 @@ Module SchIA. Section sim.
 
     (* after call - prepare for termination *)
     steps_l. rename _q into vret.
-    iMod (Hpost $ vret with "[ASM]") as "[W [[TidF [TID YIELD]] [% [% [[-> ->] Q]]]]]"; iFrame.
+    iMod ("Post" $! vret with "[ASM]") as "[W [[TidF [TID YIELD]] [% [% [[-> ->] Q]]]]]"; iFrame.
     hss_l; steps_l.
 
     steps_r. hss_r. steps_r.
@@ -147,7 +148,7 @@ Module SchIA. Section sim.
 
     steps_r. call "IST".
     clear ret st_s st_t; iIntros (ret st_s st_t) "IST". steps_l.
-    iDestruct "ASM" as "[W [TidF [-> ->]]]".
+    iDestruct "ASM" as "[TidF [-> ->]]".
     steps_r.
     by_coind CIH; eauto.
     iPoseProof (winv_split_empty with "I") as "[I E]".
@@ -160,7 +161,7 @@ Module SchIA. Section sim.
 
     (* preprocess source precondition *)
     step_l. destruct _q as [user_pre user_post]. steps_l.
-    iDestruct "ASM" as "[% [% [% [[-> [-> %Hspawn]] ASM]]]]".
+    iDestruct "ASM" as "[% [% [% [[-> ->] [Spawn ASM]]]]]".
     hss_l; hss_r.
     steps_l. steps_r.
 
@@ -196,8 +197,10 @@ Module SchIA. Section sim.
     }
     rewrite -{3}Qp.three_quarter_quarter -dfrac_op_own -{2}(agree_idemp (to_agree _)).
     iDestruct "JoinF" as "[JoinF1 JoinF2]".
-    force_l. iSplitL "ASM JoinF1 TidF".
-    { iIntros "?? $"; iFrame. iExists user_pre, _, _, fn; iFrame; iPureIntro; esplits; eauto. }
+    force_l. iSplitL "ASM JoinF1 TidF Spawn".
+    { iIntros "???"; iFrame "JoinF1 Spawn TidF".
+      iExists _, _; iFrame; iPureIntro; esplits; eauto.
+    }
     steps_l. force_l (mtid_new↑). steps_l.
     force_l. iSplitL "JoinF2".
     { iExists _; iSplit; eauto. }
@@ -229,7 +232,7 @@ Module SchIA. Section sim.
     iStartSim.
 
     step_l. destruct _q as [[stid mtid] ?]. steps_l.
-    iDestruct "ASM" as "[W [[Tid [TID YIELD]] [-> ->]]]".
+    iDestruct "ASM" as "[[Tid [TID YIELD]] [-> ->]]".
     hss_l; hss_r.
     iDestruct "IST" as "[% [%tid_cur [%stid_cur [[-> [-> %Htid_cur]] [JoinA [TidA [RET Ys]]]]]]]".
     destruct Htid_cur as [ro_cur [post_cur Htid_cur]].
@@ -272,6 +275,7 @@ Module SchIA. Section sim.
       rewrite big_sepL_delete; try iFrame.
       rewrite ?list_lookup_fmap; destruct (ths !! tidn) as [[[? ?] ?]|]; ss.
     }
+    iApply wsim_unfold; iIntros "W".
     forces_l. iFrame "W TID YIELD". steps_l.
     iApply wsim_yield; iFrame. iSplit.
     { destruct (ths !! tidn) as [[[? ?] ?]|] eqn : ?; ss; clarify.
@@ -289,7 +293,7 @@ Module SchIA. Section sim.
     iStartSim.
 
     step_l. destruct _q as [[stid mtid] post]. steps_l.
-    iDestruct "ASM" as "[W [TID [%tid [[-> ->] JoinF]]]]". hss_l; hss_r.
+    iDestruct "ASM" as "[TID [%tid [[-> ->] JoinF]]]". hss_l; hss_r.
 
     steps_r. steps_l.
     iApply wsim_reset. iStopProof.
@@ -298,7 +302,7 @@ Module SchIA. Section sim.
     eapply wsim_coind. intros g' _ CIH a.
     destruct a as [st_src st_tgt]. s.
     destruct_quant CIH.
-    iIntros "[IST [W [Tid JoinF]]]".
+    iIntros "[IST [Tid JoinF]]".
 
     unfold_iterC_l; unfold_iterC_r.
 
@@ -318,7 +322,7 @@ Module SchIA. Section sim.
       iCombine "JoinF" "JoinF2" as "JoinF"; rewrite Qp.quarter_three_quarter.
       iEval (rewrite WF agree_idemp) in "JoinF".
       iPoseProof ("RET" with "[JoinF]") as "RET"; first (iRight; iFrame).
-      forces_l. iEval (rewrite -WF) in "Post". iFrame "Tid Post W".
+      forces_l. iEval (rewrite -WF) in "Post". iFrame "Tid Post".
       iSplit; eauto.
       step. iSplit; eauto.
       iFrame. des; iExists _; iPureIntro; esplits; eauto.
@@ -326,11 +330,11 @@ Module SchIA. Section sim.
     { steps_r.
       steps_l. unshelve erewrite (lookup_weaken _ _ _ _ _ SchInSp); cycle 1.
       { rewrite /SchA.sp; simpl_map; refl. }
-      force_l (stid, mtid, tt). steps_l. force_l. force_l. iFrame "W Tid". iSplit; eauto.
+      force_l (stid, mtid, tt). steps_l. force_l. force_l. iFrame "Tid". iSplit; eauto.
       steps_l. call "JoinA TidA RET Ys".
       { iFrame. des; iExists _; iPureIntro; esplits; eauto. }
       iIntros (ret st_src st_tgt) "IST". steps_l. steps_r.
-      iDestruct "ASM" as "[W [Tid [-> ->]]]". hss_l; hss_r.
+      iDestruct "ASM" as "[Tid [-> ->]]". hss_l; hss_r.
       steps_r. steps_l.
       by_coind CIH. iFrame.
     }
