theories/modules/Sp.v
@@ -33,9 +33,9 @@ Section sp.
 
   (* Definition sp_none : specmap := const None. *)
 
-  Variant fn_has_spec (sp : specmap) (fn : string) (fsp : fspec) : Prop :=
-  | fn_has_spec_intro (WEAK : fspec_imply (fspec_flat (sp !! (speckey_fn fn))) fsp).
-  Hint Constructors fn_has_spec : core.
+  (* Variant fn_has_spec (sp : specmap) (fn : string) (fsp : fspec) : Prop :=
+  | fn_has_spec_intro (WEAK : ⊢ fspec_imply (fspec_flat (sp !! (speckey_fn fn))) fsp).
+  Hint Constructors fn_has_spec : core. *)
 
   (* Variant fn_has_spec_in (spl : spl_type) (fn : string) (fsp : fspec) : Prop :=
   | fn_has_spec_in_intro
@@ -44,11 +44,11 @@ Section sp.
       (WEAK : fspec_imply (fspec_flat fsp_real) fsp).
   Hint Constructors fn_has_spec_in : core. *)
 
-  Lemma fn_has_weaker_spec (sp : specmap) (fn : string) (fsp0 fsp1 : fspec)
+  (* Lemma fn_has_weaker_spec (sp : specmap) (fn : string) (fsp0 fsp1 : fspec)
       (SPEC : fn_has_spec sp fn fsp0)
-      (WEAK : fspec_imply fsp0 fsp1) :
+      (WEAK : ⊢ fspec_imply fsp0 fsp1) :
     fn_has_spec sp fn fsp1.
-  Proof using. inv SPEC. econs; eauto. etrans; eauto. Qed.
+  Proof using. inv SPEC. econs; eauto. etrans; eauto. Qed. *)
 
   (* Lemma fn_has_weaker_spec_in (spl : spl_type) (fn : string) (fsp0 fsp1 : fspec)
       (SPEC : fn_has_spec_in spl fn fsp0)
@@ -56,10 +56,10 @@ Section sp.
     fn_has_spec_in spl fn fsp1.
   Proof using. inv SPEC. econs; eauto. etrans; eauto. Qed. *)
 
-  Definition sp_imply (sp0 sp1 : specmap) : Prop :=
-    ∀ fn, fspec_imply (fspec_flat (sp0 !! (speckey_fn fn))) (fspec_flat (sp1 !! (speckey_fn fn))).
+  (* Definition sp_imply (sp0 sp1 : specmap) : Prop :=
+    ∀ fn, fspec_imply (fspec_flat (sp0 !! (speckey_fn fn))) (fspec_flat (sp1 !! (speckey_fn fn))). *)
 
-  Global Program Instance sp_imply_PreOrder : PreOrder sp_imply.
+  (* Global Program Instance sp_imply_PreOrder : PreOrder sp_imply.
   Next Obligation. ii. exists x1. esplits; et. Qed.
   Next Obligation.
     intros x y z Hxy Hyz fn z1. exploit Hyz; et; intros [y1 [Hypre Hypost]].
@@ -67,7 +67,7 @@ Section sp.
     exists x1. split; ii.
     - rewrite Hypre Hxpre. iIntros ">>H". et.
     - rewrite Hxpost Hypost. iIntros ">>H". et.
-  Qed.
+  Qed. *)
 
   (* Commented out since fspec_imply' erased *)
   (* Definition sp_imply' (sp0 sp1 : specmap) : Prop :=
